#set page(numbering: "1")
#import "@preview/ctheorems:1.1.3": *
#show: thmrules
#let lemma = thmbox("lemma", "Lemma", base: none)
#let theorem = thmbox("theorem", "Theorem", base: none)
#let proof = thmproof("proof", "Proof")
#set math.mat(delim: "[")
#set math.equation(numbering: "(1)")

#show math.equation: it => {
  if it.block and not it.has("label") and it.numbering != none {
    counter(math.equation).update(v => v - 1)
    
    // Fix: Create a dictionary of fields, remove 'body', 
    // and pass 'it.body' positionally.
    let fields = it.fields()
    let _ = fields.remove("body") 
    
    math.equation(it.body, ..fields, numbering: none)
  } else {
    it
  }
}

#show heading.where(level: 1): it => {
  pagebreak(weak: true)
  it
}

#outline(depth: 1)

= Artin 2.1.5 Consequences of an equation

We are given that $x y z = 1$ in some group $G$. So
$
  y z = x^(-1)
$
and therefore
$
  y z x = 1 .
$

But it is not necessarily the case that $y x z = 1$. We know $x y = z^(-1)$ but we don't know that this group is abelian.

= Artin 2.1.7 Proving that a given binary op is associative

Given the law of composition
$
  a b = a ,
$
we must prove that
$
  (a b)c = a(b c) .
$
The LHS becomes
$
  (a)c = a c = a
$
while the RHS becomes
$
  a(b) = a b = a
$
so it is proved.

= Artin 2.2.1 A cyclic matrix group

The elements of the cyclic group generated by
$
  mat(1,1;-1,0)
$
are its powers:
$
  mat(1,1;-1,0), mat(0,1;-1,-1), mat(-1,0;0,-1), mat(-1,-1;1,0), mat(0,-1;1,1),mat(1,0;0,1) .
$
So it's a cyclic group of order 6, isomorphic to the integers modulo 6.

Note that $A^3 = -I$, so $A^6 = I$ is immediate and it's easy to get $A^4 = -A$ and $A^5 = -A^2$ from previously computed powers.

= Artin 2.2.15 Uniqueness of identity and inverses in subgroups

== (a)

Let $e_H$ be the idenity in $H$. Then
$
  e_H e_H = e_H
$
but since the operation is inherited from $G$ we may multiply by $e_H^(-1)$ in $G$:
$
  e_H^(-1)e_H e_H = e_H^(-1)e_H
$
to get
$
  e_G e_H = e_G ,
$
that is,
$
  e_H = e_G .
$

== (b)

Let $a^(-H)$ be the inverse in $H$ and $a^(-G)$ be the inverse in $G$. Then in $H$ we have
$
  a a^(-H) = 1
$
but this equation holds in $G$ as well we may multiply on the left by $a^(-G)$ in $G$ to get
$
  a^(-G) a a^(-H) = a^(-G)
$
where the first two factors on the left multiply in $G$ to give the identity, so
$
  a^(-H) = a^(-G) .
$
= Artin 2.2.20(a) The order of products in abelian groups

Let $a,b$ be elements of an abelian group of orders $m,n$ respectively. Then
$
  a^m = e
$
and
$
  b^n = e .
$

If
$
  (a b)^l = e
$
then
$
  a^l b^l = e
$
